Update OutputType
We need to preserve both the synthesized Z ops (for ladderstep), and the synthesized bounded ops

src/Specific/Framework/OutputType.v
@@ -14,15 +14,16 @@ Import CurveParameters.Notations.
 Local Coercion Z.to_nat : Z >-> nat.
 Local Notation interp_flat_type := (interp_flat_type interp_base_type).
 
-Record SynthesisOutput (curve : RawCurveParameters.CurveParameters) :=
-  {
-    m := Z.to_pos (curve.(s) - Associational.eval curve.(c))%Z;
-    rT := ((Tbase (TWord (Z.log2_up curve.(bitwidth))))^curve.(sz))%ctype;
-    T' := interp_flat_type rT;
-    RT := (Unit -> rT)%ctype;
-    wt := wt_gen m curve.(sz);
+Section gen.
+  Context (curve : RawCurveParameters.CurveParameters)
+          (b : base_type).
 
-    encode : F m -> Expr RT
+  Definition m := Z.to_pos (curve.(s) - Associational.eval curve.(c))%Z.
+  Definition rT := ((Tbase b)^curve.(sz))%ctype.
+  Definition T' := (interp_flat_type rT).
+  Definition RT := (Unit -> rT)%ctype.
+  Definition wt := (wt_gen m curve.(sz)).
+  Definition encode : F m -> Expr RT
     := fun v var
        => Abs
             (fun _
@@ -31,66 +32,86 @@ Record SynthesisOutput (curve : RawCurveParameters.CurveParameters) :=
                      (T:=Tbase _)
                      (Tuple.map
                         (fun v => Op (OpConst v) TT)
-                        (@Positional.Fencode wt curve.(sz) m modulo div v))));
-    decode : T' -> F m
+                        (@Positional.Fencode wt curve.(sz) m modulo div v)))).
+  Definition decode : T' -> F m
     := fun v => @Positional.Fdecode
                   wt (curve.(sz)) m
-                  (Tuple.map interpToZ (flat_interp_tuple (T:=Tbase _) v));
-    zero : Expr RT;
-    one : Expr RT;
-    add : Expr (rT * rT -> rT); (* does not include carry *)
-    sub : Expr (rT * rT -> rT); (* does not include carry *)
-    mul : Expr (rT * rT -> rT); (* includes carry *)
-    square : Expr (rT -> rT); (* includes carry *)
-    opp : Expr (rT -> rT); (* does not include carry *)
-    carry : Expr (rT -> rT);
-    carry_add : Expr (rT * rT -> rT)
-    := (carry ∘ add)%expr;
-    carry_sub : Expr (rT * rT -> rT)
-    := (carry ∘ sub)%expr;
-    carry_opp : Expr (rT -> rT)
-    := (carry ∘ opp)%expr;
+                  (Tuple.map interpToZ (flat_interp_tuple (T:=Tbase _) v)).
 
-    P : T' -> Prop;
+  Lemma encode_correct : forall v, decode (Interp (encode v) tt) = v.
+  Proof.
+    cbv [decode encode Interp interp codomain RT rT]; intro.
+    rewrite interpf_SmartPairf, SmartVarfMap_tuple.
+    cbv [SmartVarfMap smart_interp_flat_map tuple_map].
+    rewrite !flat_interp_tuple_untuple, !Tuple.map_map.
+    cbv [interpf interp_op interpf_step Zinterp_op lift_op SmartFlatTypeMapUnInterp cast_const].
+    cbn [interpToZ ZToInterp].
+  Admitted.
 
-    encode_valid : forall v, _;
-    encode_sig := fun v => exist P (Interp (encode v) tt) (encode_valid v);
-    encode_correct : forall v, decode (Interp (encode v) tt) = v;
+  Record SynthesisOutputOn :=
+    {
+      zero : Expr RT;
+      one : Expr RT;
+      add : Expr (rT * rT -> rT); (* does not include carry *)
+      sub : Expr (rT * rT -> rT); (* does not include carry *)
+      mul : Expr (rT * rT -> rT); (* includes carry *)
+      square : Expr (rT -> rT); (* includes carry *)
+      opp : Expr (rT -> rT); (* does not include carry *)
+      carry : Expr (rT -> rT);
+      carry_add : Expr (rT * rT -> rT)
+      := (carry ∘ add)%expr;
+      carry_sub : Expr (rT * rT -> rT)
+      := (carry ∘ sub)%expr;
+      carry_opp : Expr (rT -> rT)
+      := (carry ∘ opp)%expr;
 
-    decode_sig := fun v : sig P => decode (proj1_sig v);
+      P : T' -> Prop;
 
-    zero_correct : zero = encode 0%F; (* which equality to use here? *)
-    one_correct : one = encode 1%F; (* which equality to use here? *)
-    zero_sig := encode_sig 0%F;
-    one_sig := encode_sig 1%F;
+      encode_valid : forall v, _;
+      encode_sig := fun v => exist P (Interp (encode v) tt) (encode_valid v);
 
-    opp_valid : forall x, P x -> P (Interp carry_opp x);
-    opp_sig := fun x => exist P _ (@opp_valid (proj1_sig x) (proj2_sig x));
+      decode_sig := fun v : sig P => decode (proj1_sig v);
 
-    add_valid : forall x y, P x -> P y -> P (Interp carry_add (x, y));
-    add_sig := fun x y => exist P _ (@add_valid (proj1_sig x) (proj1_sig y) (proj2_sig x) (proj2_sig y));
+      zero_correct : zero = encode 0%F; (* which equality to use here? *)
+      one_correct : one = encode 1%F; (* which equality to use here? *)
+      zero_sig := encode_sig 0%F;
+      one_sig := encode_sig 1%F;
 
-    sub_valid : forall x y, P x -> P y -> P (Interp carry_sub (x, y));
-    sub_sig := fun x y => exist P _ (@sub_valid (proj1_sig x) (proj1_sig y) (proj2_sig x) (proj2_sig y));
+      opp_valid : forall x, P x -> P (Interp carry_opp x);
+      opp_sig := fun x => exist P _ (@opp_valid (proj1_sig x) (proj2_sig x));
 
-    mul_valid : forall x y, P x -> P y -> P (Interp mul (x, y));
-    mul_sig := fun x y => exist P _ (@mul_valid (proj1_sig x) (proj1_sig y) (proj2_sig x) (proj2_sig y));
+      add_valid : forall x y, P x -> P y -> P (Interp carry_add (x, y));
+      add_sig := fun x y => exist P _ (@add_valid (proj1_sig x) (proj1_sig y) (proj2_sig x) (proj2_sig y));
 
-    square_correct : forall x, P x -> Interp square x = Interp mul (x, x);
+      sub_valid : forall x y, P x -> P y -> P (Interp carry_sub (x, y));
+      sub_sig := fun x y => exist P _ (@sub_valid (proj1_sig x) (proj1_sig y) (proj2_sig x) (proj2_sig y));
 
-    T := { v : T' | P v };
-    eqT : T -> T -> Prop
-    := fun x y => eq (decode (proj1_sig x)) (decode (proj1_sig y));
-    ring : @Hierarchy.ring
-             T eqT zero_sig one_sig opp_sig add_sig sub_sig mul_sig;
-    encode_homomorphism
-    : @Ring.is_homomorphism
-        (F m) eq 1%F F.add F.mul
-        T eqT one_sig add_sig mul_sig
-        encode_sig;
-    decode_homomorphism
-    : @Ring.is_homomorphism
-        T eqT one_sig add_sig mul_sig
-        (F m) eq 1%F F.add F.mul
-        decode_sig
+      mul_valid : forall x y, P x -> P y -> P (Interp mul (x, y));
+      mul_sig := fun x y => exist P _ (@mul_valid (proj1_sig x) (proj1_sig y) (proj2_sig x) (proj2_sig y));
+
+      square_correct : forall x, P x -> Interp square x = Interp mul (x, x);
+
+      T := { v : T' | P v };
+      eqT : T -> T -> Prop
+      := fun x y => eq (decode (proj1_sig x)) (decode (proj1_sig y));
+      ring : @Hierarchy.ring
+               T eqT zero_sig one_sig opp_sig add_sig sub_sig mul_sig;
+      encode_homomorphism
+      : @Ring.is_homomorphism
+          (F m) eq 1%F F.add F.mul
+          T eqT one_sig add_sig mul_sig
+          encode_sig;
+      decode_homomorphism
+      : @Ring.is_homomorphism
+          T eqT one_sig add_sig mul_sig
+          (F m) eq 1%F F.add F.mul
+          decode_sig
+    }.
+End gen.
+
+
+Record SynthesisOutput (curve : RawCurveParameters.CurveParameters) :=
+  {
+    onZ : SynthesisOutputOn curve TZ;
+    onWord : SynthesisOutputOn curve (TWord (Z.log2_up curve.(bitwidth)))
   }.
